WIP

proof/MatchSimModSemExcl2.v
@@ -10,14 +10,31 @@ Set Implicit Arguments.
 
 
 
+Set Typeclasses Iterative Deepening.
+Class LeibEq (A B: Type) := { leibeq: A = B }.
+Arguments LeibEq: clear implicits.
+Definition cast_sigT (a: {ty: Type & ty}) (B: Type) `{LeibEq (projT1 a) B}: B.
+  rewrite <- leibeq. destruct a. simpl. auto.
+Defined.
+Global Program Instance LeibEq_rev (A B: Type) `{LeibEq A B}: LeibEq B A.
+Next Obligation. rewrite leibeq. eauto. Defined.
+Definition cast (A B: Type) `{LeibEq A B} (a: A): B. rewrite <- leibeq. apply a. Defined.
+Global Program Instance LeibEq_refl (A: Type): LeibEq A A.
+Global Program Instance LeibEq_fun (A B: Type) `{LeibEq A B} f: LeibEq (f A) (f B).
+Next Obligation. destruct H. subst. auto. Defined.
+
 
 
 Section MATCHSIMFORWARD.
 
-  Context {SM: SimMem.class} {SS: SimSymb.class SM} {SU: Sound.class}.
-  Context {SML: SimMemLift.class SM}.
+  Context {owned_heap_src owned_heap_tgt: Type}.
+  Context `{SMO: SimMemOh.class owned_heap_src owned_heap_tgt}
+          {SS: SimSymb.class SM} {SU: Sound.class}.
+  Context {SMOL: SimMemOhLift.class SMO}.
 
   Variable msp: ModSemPair.t.
+  Variable OHSRC: (LeibEq owned_heap_src msp.(ModSemPair.src).(ModSem.owned_heap)).
+  Variable OHTGT: (LeibEq owned_heap_tgt msp.(ModSemPair.tgt).(ModSem.owned_heap)).
   Variable index: Type.
   Variable order: index -> index -> Prop.
   Hypothesis WFORD: well_founded order.
@@ -29,100 +46,102 @@ Section MATCHSIMFORWARD.
   Hypothesis PRSV: forall si, local_preservation ms_src (sound_states si).
 
   Variable match_states: forall
-      (idx: index) (st_src0: ms_src.(ModSem.state)) (st_tgt0: ms_tgt.(ModSem.state)) (sm0: SimMem.t),
+      (idx: index) (st_src0: ms_src.(ModSem.state)) (st_tgt0: ms_tgt.(ModSem.state)) (smo0: SimMemOh.t),
       Prop.
 
   Variable match_states_at: forall
-      (st_src0: ms_src.(ModSem.state)) (st_tgt0: ms_tgt.(ModSem.state)) (sm_at sm_arg: SimMem.t),
+      (st_src0: ms_src.(ModSem.state)) (st_tgt0: ms_tgt.(ModSem.state)) (sm_at sm_arg: SimMemOh.t),
       Prop.
 
   Inductive match_states_at_helper
-            (idx_at: index) (st_src0: ms_src.(ModSem.state)) (st_tgt0: ms_tgt.(ModSem.state)) (sm_at sm_arg: SimMem.t): Prop :=
+            (idx_at: index) (st_src0: ms_src.(ModSem.state)) (st_tgt0: ms_tgt.(ModSem.state)) (smo_at smo_arg: SimMemOh.t): Prop :=
   | match_states_at_intro
-      (MATCH: match_states idx_at st_src0 st_tgt0 sm_at)
-      args_src args_tgt
-      (CALLSRC: ms_src.(ModSem.at_external) st_src0 args_src)
-      (CALLTGT: ms_tgt.(ModSem.at_external) st_tgt0 args_tgt)
-      (SIMARGS: SimMem.sim_args args_src args_tgt sm_arg)
-      (MLE: SimMem.le sm_at sm_arg)
-      (MWF: SimMem.wf sm_arg)
-      (MATCHARG: match_states_at st_src0 st_tgt0 sm_at sm_arg).
-      (* (FOOT: has_footprint st_src0 st_tgt0 sm_at) *)
+      (MATCH: match_states idx_at st_src0 st_tgt0 smo_at)
+      oh_src oh_tgt args_src args_tgt
+      (CALLSRC: ms_src.(ModSem.at_external) st_src0 oh_src args_src)
+      (CALLTGT: ms_tgt.(ModSem.at_external) st_tgt0 oh_tgt args_tgt)
+      (SIMARGS: SimMemOh.sim_args (cast oh_src) (cast oh_tgt) args_src args_tgt smo_arg)
+      (MLE: SimMem.le smo_at smo_arg)
+      (MWF: SimMem.wf smo_arg)
+      (MATCHARG: match_states_at st_src0 st_tgt0 smo_at smo_arg).
+      (* (FOOT: has_footprint st_src0 st_tgt0 smo_at) *)
 
   Hypothesis INITBSIM: forall
-      sm_arg args_src args_tgt st_init_tgt
-      (SIMSKENV: ModSemPair.sim_skenv msp sm_arg)
-      (MWF: SimMem.wf sm_arg)
-      (SIMARGS: SimMem.sim_args args_src args_tgt sm_arg)
-      (INITTGT: ms_tgt.(ModSem.initial_frame) args_tgt st_init_tgt)
-      (SAFESRC: exists _st_init_src, ms_src.(ModSem.initial_frame) args_src _st_init_src),
-      exists st_init_src sm_init idx_init,
-        (<<INITSRC: ms_src.(ModSem.initial_frame) args_src st_init_src>>) /\
-        (<<MLE: SimMem.le sm_arg sm_init>>) /\
-        (<<MATCH: match_states idx_init st_init_src st_init_tgt sm_init>>).
+      oh_src oh_tgt (smo_arg: SimMemOh.t) args_src args_tgt st_init_tgt
+      (SIMSKENV: ModSemPair.sim_skenv msp smo_arg)
+      (MWF: SimMemOh.wf smo_arg)
+      (SIMARGS: SimMemOh.sim_args (cast oh_src) (cast oh_tgt) args_src args_tgt smo_arg)
+      (INITTGT: ms_tgt.(ModSem.initial_frame) oh_tgt args_tgt st_init_tgt)
+      (SAFESRC: exists _st_init_src, ms_src.(ModSem.initial_frame) oh_src args_src _st_init_src),
+      exists st_init_src smo_init idx_init,
+        (<<INITSRC: ms_src.(ModSem.initial_frame) oh_src args_src st_init_src>>) /\
+        (<<MLE: SimMemOh.le smo_arg smo_init>>) /\
+        (<<MATCH: match_states idx_init st_init_src st_init_tgt smo_init>>).
 
-  Hypothesis INITPROGRESS: forall sm_arg args_src args_tgt
-      (SIMSKENV: ModSemPair.sim_skenv msp sm_arg)
-      (MWF: SimMem.wf sm_arg)
-      (SIMARGS: SimMem.sim_args args_src args_tgt sm_arg)
-      (SAFESRC: exists st_init_src, ms_src.(ModSem.initial_frame) args_src st_init_src),
-      exists st_init_tgt, (<<INITTGT: ms_tgt.(ModSem.initial_frame) args_tgt st_init_tgt>>).
+  Hypothesis INITPROGRESS: forall (smo_arg: SimMemOh.t) oh_src oh_tgt args_src args_tgt
+      (SIMSKENV: ModSemPair.sim_skenv msp smo_arg)
+      (MWF: SimMemOh.wf smo_arg)
+      (SIMARGS: SimMemOh.sim_args (cast oh_src) (cast oh_tgt) args_src args_tgt smo_arg)
+      (SAFESRC: exists st_init_src, ms_src.(ModSem.initial_frame) oh_src args_src st_init_src),
+      exists st_init_tgt, (<<INITTGT: ms_tgt.(ModSem.initial_frame) oh_tgt args_tgt st_init_tgt>>).
 
-  Hypothesis ATMWF: forall idx0 st_src0 st_tgt0 sm0
-      (MATCH: match_states idx0 st_src0 st_tgt0 sm0)
+  Hypothesis ATMWF: forall idx0 st_src0 st_tgt0 smo0
+      (MATCH: match_states idx0 st_src0 st_tgt0 smo0)
       (CALLSRC: ms_src.(ModSem.is_call) st_src0),
-      <<MWF: SimMem.wf sm0>>.
+      <<MWF: SimMemOh.wf smo0>>.
 
-  Hypothesis ATFSIM: forall idx0 st_src0 st_tgt0 sm0 args_src
-      (SIMSKENV: ModSemPair.sim_skenv msp sm0)
-      (MATCH: match_states idx0 st_src0 st_tgt0 sm0)
-      (CALLSRC: ms_src.(ModSem.at_external) st_src0 args_src)
+  Hypothesis ATFSIM: forall idx0 st_src0 st_tgt0 (smo0: SimMemOh.t) oh_src args_src
+      (SIMSKENV: ModSemPair.sim_skenv msp smo0)
+      (MATCH: match_states idx0 st_src0 st_tgt0 smo0)
+      (CALLSRC: ms_src.(ModSem.at_external) st_src0 oh_src args_src)
       (SOUND: forall si, exists su0 m_init, (sound_states si) su0 m_init st_src0),
-      exists args_tgt sm_arg,
-        (<<CALLTGT: ms_tgt.(ModSem.at_external) st_tgt0 args_tgt>>) /\
-        (<<SIMARGS: SimMem.sim_args args_src args_tgt sm_arg>>) /\
-        (<<MLE: SimMem.le sm0 sm_arg>>) /\
-        (<<MWF: SimMem.wf sm_arg>>) /\
-        (<<MATCHAT: match_states_at st_src0 st_tgt0 sm0 sm_arg>>).
+      exists oh_tgt args_tgt smo_arg,
+        (<<CALLTGT: ms_tgt.(ModSem.at_external) st_tgt0 oh_tgt args_tgt>>) /\
+        (<<SIMARGS: SimMemOh.sim_args (cast oh_src) (cast oh_tgt) args_src args_tgt smo_arg>>) /\
+        (<<MLE: SimMemOh.le smo0 smo_arg>>) /\
+        (<<MWF: SimMemOh.wf smo_arg>>) /\
+        (<<MATCHAT: match_states_at st_src0 st_tgt0 smo0 smo_arg>>).
 
-  Hypothesis AFTERFSIM: forall idx0 st_src0 st_tgt0 sm0 sm_arg sm_ret retv_src retv_tgt st_src1
-      (SIMSKENV: ModSemPair.sim_skenv msp sm0)
-      (MATCH: match_states idx0 st_src0 st_tgt0 sm0)
-      (MLE: SimMem.le sm0 sm_arg)
-      (* (MWF: SimMem.wf sm_arg) *)
-      (MLE: SimMem.le (SimMemLift.lift sm_arg) sm_ret)
-      (MWF: SimMem.wf sm_ret)
-      (SIMRET: SimMem.sim_retv retv_src retv_tgt sm_ret)
-      (AFTERSRC: ms_src.(ModSem.after_external) st_src0 retv_src st_src1)
+  Hypothesis AFTERFSIM: forall
+      idx0 st_src0 st_tgt0 (smo0: SimMemOh.t) smo_arg smo_ret
+      oh_src oh_tgt retv_src retv_tgt st_src1
+      (SIMSKENV: ModSemPair.sim_skenv msp smo0)
+      (MATCH: match_states idx0 st_src0 st_tgt0 smo0)
+      (MLE: SimMemOh.le smo0 smo_arg)
+      (* (MWF: SimMemOh.wf smo_arg) *)
+      (MLE: SimMemOh.le (SimMemOhLift.lift smo_arg) smo_ret)
+      (MWF: SimMemOh.wf smo_ret)
+      (SIMRET: SimMemOh.sim_retv (cast oh_src) (cast oh_tgt) retv_src retv_tgt smo_ret)
+      (AFTERSRC: ms_src.(ModSem.after_external) st_src0 oh_src retv_src st_src1)
       (SOUND: forall si, exists su0 m_init, (sound_states si) su0 m_init st_src0)
 
       (* history *)
-      (HISTORY: match_states_at_helper idx0 st_src0 st_tgt0 sm0 sm_arg)
+      (HISTORY: match_states_at_helper idx0 st_src0 st_tgt0 smo0 smo_arg)
 
       (* just helpers *)
-      (MWFAFTR: SimMem.wf (SimMemLift.unlift sm_arg sm_ret))
-      (MLEAFTR: SimMem.le sm_arg (SimMemLift.unlift sm_arg sm_ret)),
-      exists sm_after idx1 st_tgt1,
-        (<<MLE: SimMem.le sm0 sm_after>>) /\
-        forall (MLE: SimMem.le sm0 sm_after) (* helper *),
-          ((<<AFTERTGT: ms_tgt.(ModSem.after_external) st_tgt0 retv_tgt st_tgt1>>) /\
-           (<<MATCH: match_states idx1 st_src1 st_tgt1 sm_after>>)).
+      (MWFAFTR: SimMemOh.wf (SimMemOhLift.unlift smo_arg smo_ret))
+      (MLEAFTR: SimMemOh.le smo_arg (SimMemOhLift.unlift smo_arg smo_ret)),
+      exists smo_after idx1 st_tgt1,
+        (<<MLE: SimMemOh.le smo0 smo_after>>) /\
+        forall (MLE: SimMemOh.le smo0 smo_after) (* helper *),
+          ((<<AFTERTGT: ms_tgt.(ModSem.after_external) st_tgt0 oh_tgt retv_tgt st_tgt1>>) /\
+           (<<MATCH: match_states idx1 st_src1 st_tgt1 smo_after>>)).
 
-  Hypothesis FINALFSIM: forall idx0 st_src0 st_tgt0 sm0 retv_src
-      (SIMSKENV: ModSemPair.sim_skenv msp sm0)
-      (MATCH: match_states idx0 st_src0 st_tgt0 sm0)
-      (FINALSRC: ms_src.(ModSem.final_frame) st_src0 retv_src),
-      exists sm_ret retv_tgt,
-        (<<FINALTGT: ms_tgt.(ModSem.final_frame) st_tgt0 retv_tgt>>) /\
-        (<<SIMRET: SimMem.sim_retv retv_src retv_tgt sm_ret>>) /\
-        (<<MLE: SimMem.le sm0 sm_ret>>) /\
-        (<<MWF: SimMem.wf sm_ret>>).
+  Hypothesis FINALFSIM: forall idx0 st_src0 st_tgt0 (smo0: SimMemOh.t) oh_src retv_src
+      (SIMSKENV: ModSemPair.sim_skenv msp smo0)
+      (MATCH: match_states idx0 st_src0 st_tgt0 smo0)
+      (FINALSRC: ms_src.(ModSem.final_frame) st_src0 oh_src retv_src),
+      exists smo_ret oh_tgt retv_tgt,
+        (<<FINALTGT: ms_tgt.(ModSem.final_frame) st_tgt0 oh_tgt retv_tgt>>) /\
+        (<<SIMRET: SimMemOh.sim_retv (cast oh_src) (cast oh_tgt) retv_src retv_tgt smo_ret>>) /\
+        (<<MLE: SimMemOh.le smo0 smo_ret>>) /\
+        (<<MWF: SimMemOh.wf smo_ret>>).
 
-  Let STEPFSIM := forall idx0 st_src0 st_tgt0 sm0
-      (SIMSKENV: ModSemPair.sim_skenv msp sm0)
+  Let STEPFSIM := forall idx0 st_src0 st_tgt0 (smo0: SimMemOh.t)
+      (SIMSKENV: ModSemPair.sim_skenv msp smo0)
       (NOTCALL: ~ ModSem.is_call ms_src st_src0)
       (NOTRET: ~ ModSem.is_return ms_src st_src0)
-      (MATCH: match_states idx0 st_src0 st_tgt0 sm0)
+      (MATCH: match_states idx0 st_src0 st_tgt0 smo0)
       (SOUND: forall si, exists su0 m_init, (sound_states si) su0 m_init st_src0),
       (<<RECEP: receptive_at ms_src st_src0>>) /\
       (<<STEPFSIM: forall tr st_src1
@@ -130,15 +149,15 @@ Section MATCHSIMFORWARD.
              exists idx1 st_tgt1 sm1,
                (<<PLUS: DPlus ms_tgt st_tgt0 tr st_tgt1>> \/
                            <<STAR: DStar ms_tgt st_tgt0 tr st_tgt1 /\ order idx1 idx0>>)
-               /\ (<<MLE: SimMem.le sm0 sm1>>)
-               (* Note: We require le for mle_preserves_sim_ge, but we cannot require SimMem.wf, beacuse of DCEproof *)
+               /\ (<<MLE: SimMemOh.le smo0 sm1>>)
+               (* Note: We require le for mle_preserves_sim_ge, but we cannot require SimMemOh.wf, beacuse of DCEproof *)
                /\ (<<MATCH: match_states idx1 st_src1 st_tgt1 sm1>>)>>).
 
-  Let STEPBSIM := forall idx0 st_src0 st_tgt0 sm0
-      (SIMSKENV: ModSemPair.sim_skenv msp sm0)
+  Let STEPBSIM := forall idx0 st_src0 st_tgt0 (smo0: SimMemOh.t)
+      (SIMSKENV: ModSemPair.sim_skenv msp smo0)
       (NOTCALL: ~ ModSem.is_call ms_src st_src0)
       (NOTRET: ~ ModSem.is_return ms_src st_src0)
-      (MATCH: match_states idx0 st_src0 st_tgt0 sm0)
+      (MATCH: match_states idx0 st_src0 st_tgt0 smo0)
       (SOUND: forall si, exists su0 m_init, (sound_states si) su0 m_init st_src0),
       (<<PROGRESS: safe_modsem ms_src st_src0 -> ModSem.is_step ms_tgt st_tgt0>>) /\
       (<<STEPBSIM: forall tr st_tgt1
@@ -146,8 +165,8 @@ Section MATCHSIMFORWARD.
              exists idx1 st_src1 sm1,
                (<<PLUS: Plus ms_src st_src0 tr st_src1>> \/
                            <<STAR: Star ms_src st_src0 tr st_src1 /\ order idx1 idx0>>)
-               /\ (<<MLE: SimMem.le sm0 sm1>>)
-               (* Note: We require le for mle_preserves_sim_ge, but we cannot require SimMem.wf, beacuse of DCEproof *)
+               /\ (<<MLE: SimMemOh.le smo0 sm1>>)
+               (* Note: We require le for mle_preserves_sim_ge, but we cannot require SimMemOh.wf, beacuse of DCEproof *)
                /\ (<<MATCH: match_states idx1 st_src1 st_tgt1 sm1>>)>>).
 
   Hypothesis STEPSIM: STEPFSIM \/ STEPBSIM.
@@ -155,16 +174,17 @@ Section MATCHSIMFORWARD.
   Hypothesis BAR: bar_True.
 
   Lemma match_states_lxsim
-        sm_init i0 st_src0 st_tgt0 sm0
-        (SIMSKENV: ModSemPair.sim_skenv msp sm0)
-        (MLE: SimMem.le sm_init sm0)
-        (* (MWF: SimMem.wf sm0) *)
-        (* (MCOMPAT: mem_compat st_src0 st_tgt0 sm0) *)
-        (MATCH: match_states i0 st_src0 st_tgt0 sm0):
+        smo_init i0 st_src0 st_tgt0 (smo0: SimMemOh.t)
+        (SIMSKENV: ModSemPair.sim_skenv msp smo0)
+        (MLE: SimMemOh.le smo_init smo0)
+        (* (MWF: SimMemOh.wf smo0) *)
+        (* (MCOMPAT: mem_compat st_src0 st_tgt0 smo0) *)
+        (MATCH: match_states i0 st_src0 st_tgt0 smo0):
         (* su0 *)
-      (* <<LXSIM: lxsim ms_src ms_tgt (sound_state su0) sm_init i0.(to_idx WFORD) st_src0 st_tgt0 sm0>> *)
-      <<LXSIM: lxsim ms_src ms_tgt (fun st => forall si, exists su0 m_init, sound_states si su0 m_init st)
-                     (Ord.lift_idx WFORD i0) st_src0 st_tgt0 sm0>>.
+      (* <<LXSIM: lxsim ms_src ms_tgt (sound_state su0) smo_init i0.(to_idx WFORD) st_src0 st_tgt0 smo0>> *)
+      <<LXSIM: lxsim (SMO:=cast SMO)
+                     ms_src ms_tgt (fun st => forall si, exists su0 m_init, sound_states si su0 m_init st)
+                     (Ord.lift_idx WFORD i0) st_src0 st_tgt0 smo0>>.
   Proof.
     (* move su0 at top. *)
     revert_until BAR. pcofix CIH. i. pfold. ii.
@@ -174,16 +194,16 @@ Section MATCHSIMFORWARD.
         exploit ATMWF; eauto. i; des. ii. eapply lxsim_at_external; eauto. ii. clear CALLSRC.
         exploit ATFSIM; eauto. { ii. eapply SUSTAR; eauto. eapply star_refl. } i; des.
         (* determ_tac ModSem.at_external_dtm. clear_tac. *)
-        eexists _, (SimMemLift.lift sm_arg).
+        eexists _, (SimMemOhLift.lift smo_arg).
         esplits; eauto.
-        { eapply SimMemLift.lift_args; eauto. }
-        { eapply SimMemLift.lift_wf; eauto. }
-        { etrans; eauto. eapply SimMemLift.lift_priv; eauto. }
+        { eapply SimMemOhLift.lift_args; eauto. }
+        { eapply SimMemOhLift.lift_wf; eauto. }
+        { etrans; eauto. eapply SimMemOhLift.lift_priv; eauto. }
         i. exploit AFTERFSIM; try apply SAFESRC; try apply SIMRET; eauto.
         { ii. eapply SUSTAR. eapply star_refl. }
         { econs; eauto. }
-        { eapply SimMemLift.unlift_wf; eauto. }
-        { eapply SimMemLift.lift_spec; eauto. }
+        { eapply SimMemOhLift.unlift_wf; eauto. }
+        { eapply SimMemOhLift.lift_spec; eauto. }
         i; des. spc H1. des. esplits; eauto. right. eapply CIH; eauto.
         { eapply ModSemPair.mfuture_preserves_sim_skenv; try apply SIMSKENV; eauto.
           apply rtc_once. left. et.
@@ -221,7 +241,7 @@ Section MATCHSIMFORWARD.
     { i. eapply local_preservation_noguarantee_weak; eauto. }
     ii; ss. folder.
     exploit SimSymb.sim_skenv_func_bisim; eauto. { apply SIMSKENV. } intro FSIM; des.
-    inv FSIM. exploit FUNCFSIM; eauto. { apply SimMem.sim_args_sim_fptr; et. } i; des.
+    inv FSIM. exploit FUNCFSIM; eauto. { apply SimMemOh.sim_args_sim_fptr; et. } i; des.
     split; ii.
     - exploit INITBSIM; eauto. i; des.
       esplits; eauto.
