proof/SimMemLift.v
@@ -20,92 +20,94 @@ Set Implicit Arguments.
 
 (* A special instance of private transition, for backward compatibility *)
 
-Module SimMemLift.
+Module SimMemOhLift.
 
   (* Context `{SM: SimMem.class}. *)
 
-  Class class (SM: SimMem.class) :=
-  { lepriv_Trans :> Transitive SimMem.lepriv;
+  Class class (owned_heap_src owned_heap_tgt: Type)
+        `(SMO: SimMemOh.class owned_heap_src owned_heap_tgt) :=
+  { lepriv_Trans :> Transitive SimMemOh.lepriv;
 
-    lift: SimMem.t -> SimMem.t;
-    unlift: SimMem.t -> SimMem.t -> SimMem.t;
+    lift: SimMemOh.t -> SimMemOh.t;
+    unlift: SimMemOh.t -> SimMemOh.t -> SimMemOh.t;
 
-    lift_wf: forall mrel, SimMem.wf mrel -> SimMem.wf (lift mrel);
+    lift_wf: forall mrel, SimMemOh.wf mrel -> SimMemOh.wf (lift mrel);
     lift_src: forall mrel, (lift mrel).(SimMem.src) = mrel.(SimMem.src);
     lift_tgt: forall mrel, (lift mrel).(SimMem.tgt) = mrel.(SimMem.tgt);
     unlift_src: forall mrel0 mrel1, (unlift mrel0 mrel1).(SimMem.src) = mrel1.(SimMem.src);
     unlift_tgt: forall mrel0 mrel1, (unlift mrel0 mrel1).(SimMem.tgt) = mrel1.(SimMem.tgt);
-    lift_spec: forall mrel0 mrel1, SimMem.le (lift mrel0) mrel1 -> SimMem.wf mrel0 -> SimMem.le mrel0 (unlift mrel0 mrel1);
+    lift_spec: forall mrel0 mrel1, SimMemOh.le (lift mrel0) mrel1 -> SimMemOh.wf mrel0 -> SimMemOh.le mrel0 (unlift mrel0 mrel1);
     unlift_wf: forall mrel0 mrel1,
-        SimMem.wf mrel0 -> SimMem.wf mrel1 -> SimMem.le (lift mrel0) mrel1 -> SimMem.wf (unlift mrel0 mrel1);
+        SimMemOh.wf mrel0 -> SimMemOh.wf mrel1 -> SimMemOh.le (lift mrel0) mrel1 -> SimMemOh.wf (unlift mrel0 mrel1);
 
-    lift_sim_val: forall mrel, SimMem.sim_val mrel <2= SimMem.sim_val (lift mrel);
+    lift_sim_val: forall (mrel: SimMemOh.t), SimMem.sim_val mrel <2= SimMem.sim_val (lift mrel);
 
     (* Required for "forward" compatibility *)
 
-    lift_priv: forall sm0 (MWF: SimMem.wf sm0), SimMem.lepriv sm0 (lift sm0);
-    (* unlift_priv: forall sm0 sm1 (MWF: SimMem.wf sm0), SimMem.lepriv sm1 (unlift sm0 sm1); *)
+    lift_priv: forall sm0 (MWF: SimMemOh.wf sm0), SimMemOh.lepriv sm0 (lift sm0);
+    (* unlift_priv: forall sm0 sm1 (MWF: SimMemOh.wf sm0), SimMemOh.lepriv sm1 (unlift sm0 sm1); *)
     unlift_priv: forall
         sm_at sm_arg sm_ret
-        (MWF: SimMem.wf sm_at)
-        (MLIFT: SimMem.lepriv sm_at sm_arg)
-        (MLE: SimMem.le sm_arg sm_ret)
-        (MWF: SimMem.wf sm_ret),
-        SimMem.lepriv sm_ret (unlift sm_at sm_ret);
+        (MWF: SimMemOh.wf sm_at)
+        (MLIFT: SimMemOh.lepriv sm_at sm_arg)
+        (MLE: SimMemOh.le sm_arg sm_ret)
+        (MWF: SimMemOh.wf sm_ret),
+        SimMemOh.lepriv sm_ret (unlift sm_at sm_ret);
   }.
 
   Section PROPS.
 
-  Context {SM: SimMem.class}.
-  Context {SML: SimMemLift.class SM}.
+  Context (owned_heap_src owned_heap_tgt: Type).
+  Context `{SMO: SimMemOh.class owned_heap_src owned_heap_tgt}.
+  Context {SML: SimMemOhLift.class SMO}.
 
-  Lemma lift_sim_regset: forall sm0, SimMem.sim_regset sm0 <2= SimMem.sim_regset (SimMemLift.lift sm0).
-  Proof. ii. eapply SimMemLift.lift_sim_val; et. Qed.
+  Lemma lift_sim_regset: forall (sm0: SimMemOh.t), SimMem.sim_regset sm0 <2= SimMem.sim_regset (SimMemOhLift.lift sm0).
+  Proof. ii. eapply SimMemOhLift.lift_sim_val; et. Qed.
 
   Lemma le_lift_lepriv
         sm0 sm1 sm_lift
-        (MWF0: SimMem.wf sm0)
-        (MWF1: SimMem.wf sm1)
-        (MLE: SimMem.le sm0 sm1)
-        (MLIFT: SimMemLift.lift sm1 = sm_lift):
-      <<MLE: SimMem.lepriv sm0 sm_lift>>.
+        (MWF0: SimMemOh.wf sm0)
+        (MWF1: SimMemOh.wf sm1)
+        (MLE: SimMemOh.le sm0 sm1)
+        (MLIFT: SimMemOhLift.lift sm1 = sm_lift):
+      <<MLE: SimMemOh.lepriv sm0 sm_lift>>.
   Proof.
-    subst. hexploit (SimMemLift.lift_priv sm1); eauto. intro T. r. etrans; et.
+    subst. hexploit (SimMemOhLift.lift_priv sm1); eauto. intro T. r. etrans; et.
   Qed.
 
   Lemma lift_args
-        args_src args_tgt sm_arg0
+        args_src args_tgt (sm_arg0: SimMemOh.t)
         (ARGS: SimMem.sim_args args_src args_tgt sm_arg0):
-      <<ARGS: SimMem.sim_args args_src args_tgt (SimMemLift.lift sm_arg0)>>.
+      <<ARGS: SimMem.sim_args args_src args_tgt (SimMemOhLift.lift sm_arg0)>>.
   Proof.
     inv ARGS.
     - econs; eauto.
-      + eapply SimMemLift.lift_sim_val; et.
+      + eapply SimMemOhLift.lift_sim_val; et.
       + erewrite <- SimMem.sim_val_list_spec in *.
         eapply Forall2_impl.
-        { eapply SimMemLift.lift_sim_val; et. }
+        { eapply SimMemOhLift.lift_sim_val; et. }
         ss.
-      + rewrite SimMemLift.lift_src. ss.
-      + rewrite SimMemLift.lift_tgt. ss.
+      + rewrite SimMemOhLift.lift_src. ss.
+      + rewrite SimMemOhLift.lift_tgt. ss.
     - econs 2; eauto.
       + eapply lift_sim_regset; et.
-      + rewrite SimMemLift.lift_src. ss.
-      + rewrite SimMemLift.lift_tgt. ss.
+      + rewrite SimMemOhLift.lift_src. ss.
+      + rewrite SimMemOhLift.lift_tgt. ss.
   Qed.
 
   (* Lemma unlift_le_lepriv *)
   (*       sm_arg sm_ret sm1 *)
   (*       (MWF0: SimMem.wf sm_arg) *)
-  (*       (MWF1: SimMem.wf (SimMemLift.unlift sm_arg sm_ret)) *)
-  (*       (MLE: SimMem.le (SimMemLift.unlift sm_arg sm_ret) sm1) *)
+  (*       (MWF1: SimMem.wf (SimMemOhLift.unlift sm_arg sm_ret)) *)
+  (*       (MLE: SimMem.le (SimMemOhLift.unlift sm_arg sm_ret) sm1) *)
   (*   : *)
   (*     <<MLE: SimMem.lepriv sm_ret sm1>> *)
   (* . *)
   (* Proof. *)
-  (*   hexploit (SimMemLift.unlift_priv sm_arg sm_ret); eauto. intro T. *)
+  (*   hexploit (SimMemOhLift.unlift_priv sm_arg sm_ret); eauto. intro T. *)
   (*   r. etrans; et. *)
   (* Qed. *)
 
   End PROPS.
 
-End SimMemLift.
+End SimMemOhLift.
